![[1Q2017 - PARCIAL-1.pdf]]




# 1
## a

$$
(\alpha^{r})^{n} = (\alpha^{n})^{r}
$$
- Caso base: $n= 0 : (\alpha^{r})^{0} = (\alpha^{0})^{r}$ 
	- $(\alpha^{r})^{0} = \lambda$
	- $(\alpha^{0})^{r} = \lambda$
- HI: $(\alpha^{r})^{n} = (\alpha^{n})^{r}$
- Tesis: $(\alpha^{r})^{n+1} = (\alpha^{n+1})^{r}$

$$(\alpha^{r})^{n+1} = (\alpha^{r})^{n}(\alpha^{r})$$
Luego por HI:
$$(\alpha^{r})^{n+1} = (\alpha^{n})^{r}(\alpha^{r})$$

Que es lo mismo que 
$$(\alpha^{n+1})^{r} = (\alpha^{n}\alpha)^{r} = (\alpha^{n})^{r}(\alpha^{r})$$
## b
